Compiler/CompilationModel/ValidationInterop.lean
@@ -127,6 +127,7 @@ def validateInteropExpr (context : String) : Expr → Except String Unit
   | Expr.localVar _
   | Expr.arrayLength _ | Expr.memoryArrayLength _ | Expr.storageArrayLength _
   | Expr.paramDynamicHeadWord _ _
+  | Expr.paramDynamicStaticComposite _ _
   | Expr.paramDynamicMemberLength _ _
   | Expr.paramDynamicMemberDataOffset _ _
   | Expr.dynamicBytesEq _ _
